[minor] [verif] SFI refinement lemma -- goodness preserved.

sfi/refinementSA.v
@@ -51,15 +51,17 @@ Notation satom  := (atom word stag).
 Notation svalue := (@val word stag).
 Notation slabel := (@common.tag word stag).
 
+(* We check the compartment stuff later *)
 Definition refine_pc_b (apc : word) (spc : satom) :=
   match spc with
     | spc' @ (Sym.PC _ _) => apc == spc'
     | _                   => false
   end.
 
+(* We check the compartment stuff later *)
 Definition refine_mem_loc_b (ax : word) (sx : satom) : bool :=
   match sx with
-    | sx' @ (Sym.DATA _ I W) => is_set I && is_set W && (ax == sx')
+    | sx' @ (Sym.DATA _ _ _) => ax == sx'
     | _                      => false
   end.
 
@@ -82,7 +84,8 @@ Definition refine_compartment_b (c : Abs.compartment t)
   is_some $
     let: Abs.Compartment A J S := c in
     do! sxs <- map_options (get smem) A;
-    do! sc  <- stag_compartment =<< the (map slabel sxs); (* modulo emptiness *)
+    do! sc  <- the =<< map_options (stag_compartment ∘ slabel) sxs;
+               (* modulo emptiness *)
     do! guard? forallb (set_elem sc) <$>
                  map_options (stag_incoming ∘ slabel <=< get smem) J;
     do! guard? forallb (set_elem sc) <$>
@@ -90,22 +93,75 @@ Definition refine_compartment_b (c : Abs.compartment t)
     Some tt.
 End With_EqType_refine_compartment_b.
 
+Definition refine_compartment_set_b (C   : list (Abs.compartment t))
+                                    (sst : sstate)
+                                    (p   : word) : bool :=
+  match get (Symbolic.mem sst) p with
+    | Some (_ @ (Sym.DATA _ I W)) =>
+      is_some (assoc_list_lookup (Sym.set_ids (Symbolic.internal sst))
+                                 (eq_op I)) &&
+      is_some (assoc_list_lookup (Sym.set_ids (Symbolic.internal sst))
+                                 (eq_op W))
+    | Some (_ @ _) =>
+      false
+    | None =>
+      true
+  end.
+
 Definition refine_compartments (C : list (Abs.compartment t))
-                               (smem : smemory) : Prop :=
-  forallb (refine_compartment_b ^~ smem) C = true.
+                               (sst : sstate) : Prop :=
+  forallb (refine_compartment_b ^~ (Symbolic.mem sst)) C /\
+  (forall p, refine_compartment_set_b C sst p) /\
+  forallb (fun set_id => let: (set,id) := set_id in
+             is_set set && (id <? (Sym.next_id (Symbolic.internal sst))))
+          (Sym.set_ids (Symbolic.internal sst)).
+    (* This last condition is just what we need to guarantee that the symbolic
+       state is good if the abstract state is. *)
 
 Record refine_astate (ast : astate) (sst : sstate) : Prop := RefineState
-  { pc_refined          : refine_pc_b         (Abs.pc ast)   (Symbolic.pc sst)
+  { pc_refined          : refine_pc_b         (Abs.pc   ast) (Symbolic.pc   sst)
   ; regs_refined        : refine_registers    (Abs.regs ast) (Symbolic.regs sst)
   ; mems_refined        : refine_memory       (Abs.mem  ast) (Symbolic.mem  sst)
-  ; compartments_refine : refine_compartments (Abs.compartments ast)
-                                              (Symbolic.mem sst)}.
+  ; compartments_refine : refine_compartments (Abs.compartments ast) sst }.
 
 Inductive refine_astate' : astate' -> sstate -> Prop :=
 | refine_none : forall sst, (~ exists sst', sstep sst sst') ->
                             refine_astate' None sst
 | refine_some : forall ast sst, refine_astate ast sst ->
                                 refine_astate' (Some ast) sst.
+
+Generalizable All Variables.
+
+Theorem refine_good : forall `(REFINE : refine_astate ast sst),
+  Abs.good_state ast ->
+  Sym.good_state sst.
+Proof.
+  clear S I.
+  intros [Apc AR AM AC] [SM SR [Spc Lpc] [Snext Sids]] [RPC RREGS RMEMS RCOMPS]
+         GOOD;
+    simpl in *;
+    unfold refine_compartments in RCOMPS; simpl in RCOMPS;
+    destruct RCOMPS as [RCOMPS [RSETS ROK]];
+  unfold Sym.good_state, Abs.good_state in *; simpl in *;
+    move: GOOD => /andP [ICO GOOD].
+  repeat split.
+  - intros p; unfold Sym.good_memory_tag.
+    unfold refine_memory, pointwise in RMEMS; specialize RMEMS with p.
+    specialize RSETS with p; unfold refine_compartment_set_b in RSETS;
+      simpl in RSETS.
+    destruct (get SM p) as [[Sx SL]|] eqn:SGET; rewrite SGET in RSETS *;
+      [|trivial].
+    destruct (get AM p) as [Ax|] eqn:AGET; [simpl in RMEMS | elim RMEMS].
+    by destruct SL as [|c I W|].
+  - intros r; unfold Sym.good_register_tag.
+    unfold refine_registers, pointwise in RREGS; specialize RREGS with r.
+    destruct (get SR r) as [[Sx SL]|] eqn:SGET; rewrite SGET; [|trivial].
+    destruct (get AR r) as [Ax|] eqn:AGET; [|elim RREGS].
+    unfold refine_reg_b in RREGS.
+    by destruct SL.
+  - by destruct Lpc.
+  - exact ROK.
+Qed.
 
 Theorem backward_simulation : forall ast sst sst',
   refine_astate' ast sst ->
